simulating natives

Simulator/CoqSim/Eval.v
@@ -1,17 +1,29 @@
-Require Import Compare_dec List String.
+Require Import Compare_dec List String Streams.
 Import ListNotations.
 
 Require Import Kami.AllNotations.
+
 Require Import Kami.Simulator.CoqSim.Misc.
-Require Import Kami.Simulator.CoqSim.IO.
 Require Import Kami.Simulator.CoqSim.TransparentProofs.
+Require Import Kami.Simulator.CoqSim.SimTypes.
+Require Import Kami.Simulator.CoqSim.HaskellTypes.
+
+Section Eval.
+
+Variable Word : nat -> Type.
+Variable Vec : nat -> Type -> Type.
+Variable M : Type -> Type.
+
+Context `{IsWord Word}.
+Context `{IsVector Vec}.
+Context `{PrintMonad Word Vec M}.
 
 Fixpoint eval_Kind(k : Kind) : Type :=
   match k with
   | Bool => bool
-  | Bit n => word n
+  | Bit n => Word n
   | Struct n ks fs => Tuple (fun i => eval_Kind (ks i))
-  | Array n k' => Vec (eval_Kind k') n
+  | Array n k' => Vec n (eval_Kind k')
   end.
 
 Definition print_BF(bf : BitFormat) : nat -> string :=
@@ -24,17 +36,17 @@ Definition print_BF(bf : BitFormat) : nat -> string :=
 Fixpoint print_Kind(k : Kind)(ff : FullFormat k) : eval_Kind k -> string :=
   match ff with
   | FBool n _ => fun x => space_pad n (if x then "1" else "0")
-  | FBit n m bf => fun x => zero_pad m (print_BF bf (wordToNat x))
-  | FStruct n fk fs ffs => fun x => ("{" ++ String.concat "; " (vec_to_list (vec_map (fun '(str1,str2) => str1 ++ ":" ++ str2) (add_strings fs (tup_to_vec _ (fun i => print_Kind (ffs i)) x)))) ++ "}")%string
-  | FArray n k' ff' => fun x => ("[" ++ String.concat "; " (vec_to_list (vec_map (fun '(n,y) => nat_decimal_string n ++ "=" ++ print_Kind ff' y) (add_indices x))) ++ "]")%string (*fix*)
+  | FBit n m bf => fun x => zero_pad m (print_BF bf (word_to_nat x))
+  | FStruct n fk fs ffs => fun x => ("{" ++ String.concat "; " (v_to_list (vmap (fun '(str1,str2) => str1 ++ ":" ++ str2) (add_strings fs (tup_to_vec _ (fun i => print_Kind (ffs i)) x)))) ++ "}")%string
+  | FArray n k' ff' => fun _ => "arr" (*fix*)
   end.
 
 Fixpoint Kind_eq{k} : eval_Kind k -> eval_Kind k -> bool :=
-  match k with
+  match k return eval_Kind k -> eval_Kind k -> bool with
   | Bool => Bool.eqb
-  | Bit n => @weqb n
+  | Bit n => weqb
   | Struct n ks fs => TupEq (fun i => eval_Kind (ks i)) (fun i => @Kind_eq (ks i))
-  | Array n k' => VecEq (@Kind_eq k')
+  | Array n k' => vec_eq (@Kind_eq k')
   end.
 
 Definition eval_FK(k : FullKind) :=
@@ -43,15 +55,27 @@ Definition eval_FK(k : FullKind) :=
   | NativeKind t _ => t
   end.
 
-Fixpoint rand_val(k : Kind) : IO (eval_Kind k) :=
-  match k with
+Notation "'do' x <- y ; cont" := (bind y (fun x => cont)) (at level 20).
+
+Fixpoint rand_tuple{n} : forall ts : Fin.t n -> Type, (forall i, M (ts i)) -> M (Tuple ts) :=
+  match n with
+  | 0 => fun _ _ => ret tt
+  | S m => fun ts mxs => (
+      do x <- mxs Fin.F1;
+      do xs <- rand_tuple (fun j => ts (Fin.FS j)) (fun j => mxs (Fin.FS j));
+      ret (x,xs)
+      )
+  end.
+
+Fixpoint rand_val(k : Kind) : M (eval_Kind k) :=
+  match k return M (eval_Kind k) with
   | Bool => rand_bool
   | Bit n => rand_word n
   | Struct n ks fs => rand_tuple (fun i => eval_Kind (ks i)) (fun i => rand_val (ks i))
   | Array n k' => rand_vec (rand_val k')
   end.
 
-Fixpoint rand_val_FK(k : FullKind) : IO (eval_FK k) :=
+Fixpoint rand_val_FK(k : FullKind) : M (eval_FK k) :=
   match k with
   | SyntaxKind k' => rand_val k'
   | NativeKind k' c => ret c
@@ -69,24 +93,47 @@ Definition eval_CABool(op : CABoolOp) : list bool -> bool :=
   | Xor => fun xs => fold_left xorb xs false
   end.
 
-Definition eval_UniBit{m n}(op : UniBitOp m n) : word m -> word n :=
-  evalUniBit op.
+Definition eval_UniBit{m n}(op : UniBitOp m n) : Word m -> Word n :=
+  match op with
+  | Inv n => inv
+  | TruncLsb lsb msb => trunc_lsb
+  | TruncMsb lsb msb => trunc_msb
+  | UAnd n => uand
+  | UOr n => uor
+  | UXor n => uxor
+  end.
 
-Definition eval_BinBit{m n p}(op : BinBitOp m n p) : word m -> word n -> word p :=
-  evalBinBit op.
+Definition eval_BinBit{m n p}(op : BinBitOp m n p) : Word m -> Word n -> Word p :=
+  match op with
+  | Sub n => sub
+  | Div n => div
+  | Rem n => rem
+  | Sll n m => sll
+  | Srl n m => srl
+  | Sra n m => sra
+  | Concat msb lsb => concat
+  end.
 
-Definition eval_CABit{n}(op : CABitOp) : list (word n) -> word n :=
-  evalCABit op.
+Definition eval_CABit{n}(op : CABitOp) : list (Word n) -> Word n :=
+  match op with
+  | Add => add
+  | Mul => mul
+  | Band => band
+  | Bor => bor
+  | Bxor => bxor
+  end.
 
-Definition eval_BinBitBool{m n}(op : BinBitBoolOp m n) : word m -> word n -> bool :=
-  evalBinBitBool op.
+Definition eval_BinBitBool{m n}(op : BinBitBoolOp m n) : Word m -> Word n -> bool :=
+  match op with
+  | LessThan n => wltb
+  end.
 
 Fixpoint eval_ConstT{k}(e : ConstT k) : eval_Kind k :=
   match e with
   | ConstBool b => b
-  | ConstBit n w => w
+  | ConstBit n w => nat_to_word (wordToNat w)
   | ConstStruct n ks ss es => mkTup (fun i => eval_Kind (ks i)) (fun i => eval_ConstT (es i))
-  | ConstArray n k' es => mkVec (fun i => eval_ConstT (es i))
+  | ConstArray n k' es => make_vec (fun i => eval_ConstT (es i))
   end.
 
 Definition eval_ConstFullT{k} (e : ConstFullT k) : eval_FK k :=
@@ -100,45 +147,60 @@ Fixpoint eval_Expr{k}(e : Expr eval_Kind k) : eval_FK k :=
   | Var _ v => v
   | Const _ v => eval_ConstT v
   | UniBool op e => eval_UniBool op (eval_Expr e)
-  | CABool op es => eval_CABool op (map eval_Expr es)
+  | CABool op es => eval_CABool op (List.map eval_Expr es)
   | UniBit m n op e => eval_UniBit op (eval_Expr e)
   | BinBit m n p op e1 e2 => eval_BinBit op (eval_Expr e1) (eval_Expr e2)
-  | CABit n op es => eval_CABit op (map eval_Expr es)
+  | CABit n op es => eval_CABit op (List.map eval_Expr es)
   | BinBitBool m n op e1 e2 => eval_BinBitBool op (eval_Expr e1) (eval_Expr e2)
   | ITE _ p e1 e2 => eval_Expr (if eval_Expr p then e1 else e2)
   | Eq _ e1 e2 => Kind_eq (eval_Expr e1) (eval_Expr e2)
   | ReadStruct n ks ss e i => tup_index i _ (eval_Expr e)
   | BuildStruct n ks ss es => mkTup _ (fun i => eval_Expr (es i))
-  | ReadArray n m k v i => match lt_dec (wordToNat (eval_Expr i)) n with
-                           | left pf => vec_index (Fin.of_nat_lt pf) (eval_Expr v)
+  | ReadArray n m k v i => match lt_dec (word_to_nat (eval_Expr i)) n with
+                           | left pf => index (Fin.of_nat_lt pf) (eval_Expr v)
                            | right _ => eval_ConstT (getDefaultConst k)
                            end
-  | ReadArrayConst n k v i => vec_index i (eval_Expr v)
-  | BuildArray n k v => mkVec (fun i => eval_Expr (v i))
+  | ReadArrayConst n k v i => index i (eval_Expr v)
+  | BuildArray n k v => make_vec (fun i => eval_Expr (v i))
   end.
 
-Definition eval_SysT(s : SysT eval_Kind) : IO unit :=
+Definition eval_SysT(s : SysT eval_Kind) : M unit :=
   match s with
   | DispString s => print s
   | DispExpr k e ff => print (print_Kind ff (eval_Expr e))
   | Finish => exit
   end.
 
-Fixpoint eval_list_SysT(xs : list (SysT eval_Kind)) : IO unit :=
+Fixpoint eval_list_SysT(xs : list (SysT eval_Kind)) : M unit :=
   match xs with
   | [] => ret tt
   | s::ys => (
-      io_do _ <- eval_SysT s;
+      do _ <- eval_SysT s;
       eval_list_SysT ys
       )
   end.
 
 Section EvalAction.
 
+(* Variable KindInfo : Map string FullKind 
+Hypothesis ActionGood: forall Write r k in a, KindInfo r = k /\ forall Read r k in a, KindInfo r = k
+Lemma: SimRegGood: (r, k) in SimReg -> KindInfo r = k
+Theorem: ActionSimRegGood: forall Write r k in a, (r, k') in SimReg -> k = k' *)
+
 Definition SimReg := (string * {x : _ & fullType eval_Kind x})%type.
 Definition SimRegs := list SimReg.
 
 Variable regs : SimRegs.
+
+Record Update := {
+  reg_name : string;
+  kind : FullKind;
+  old_val : fullType eval_Kind kind;
+  new_val : fullType eval_Kind kind;
+  lookup_match : lookup String.eqb reg_name regs = Some (existT _ kind old_val)
+  }.
+
+Definition Updates := list Update.
 
 Fixpoint mkProd(ts : list Type) : Type :=
   match ts with
@@ -146,8 +208,8 @@ Fixpoint mkProd(ts : list Type) : Type :=
   | T::ts' => (T * mkProd ts')%type
   end.
 
-Fixpoint return_meth(meth : string)(sig : Signature)(meths : list (string * Signature)) : mkProd (map (fun dec => eval_Kind (fst (snd dec)) -> IO (eval_Kind (snd (snd dec)))) meths) -> option (eval_Kind (fst (sig)) -> IO (eval_Kind (snd (sig)))).
- refine match meths return mkProd (map (fun dec => eval_Kind (fst (snd dec)) -> IO (eval_Kind (snd (snd dec)))) meths) -> option (eval_Kind (fst (sig)) -> IO (eval_Kind (snd (sig)))) with
+Fixpoint return_meth(meth : string)(sig : Signature)(meths : list (string * Signature)) : mkProd (List.map (fun dec => eval_Kind (fst (snd dec)) -> M (eval_Kind (snd (snd dec)))) meths) -> option (eval_Kind (fst (sig)) -> M (eval_Kind (snd (sig)))).
+ refine match meths return mkProd (List.map (fun dec => eval_Kind (fst (snd dec)) -> M (eval_Kind (snd (snd dec)))) meths) -> option (eval_Kind (fst (sig)) -> M (eval_Kind (snd (sig)))) with
   | [] => fun _ => None
   | dec::meths' => match string_sigb (meth,sig) dec with
                    | left pf => fun fs => Some _
@@ -157,64 +219,100 @@ Fixpoint return_meth(meth : string)(sig : Signature)(meths : list (string * Sign
 Proof.
   assert (sig = snd dec).
   rewrite <- pf; auto.
-  rewrite H.
+  rewrite H4.
   exact (fst fs).
 Defined.
 
-Fixpoint eval_ActionT{k}(meths : list (string * Signature))(updates : SimRegs)(a : ActionT eval_Kind k)(fs : mkProd (map (fun dec => eval_Kind (fst (snd dec)) -> IO (eval_Kind (snd (snd dec)))) meths)){struct a} : IO (SimRegs * eval_Kind k).
-  refine match a with
-  | MCall meth s e cont => match return_meth meth s meths fs with
+Definition reg_not_found{X} : string -> M X :=
+  fun reg => error ("register " ++ reg ++ " not found.").
+
+Fixpoint wf_action{k}(a : ActionT eval_Kind k) : Prop :=
+  match a with
+  | MCall meth s e cont => forall x, wf_action (cont x)
+  | LetExpr k e cont => forall x, wf_action (cont x)
+  | LetAction k a cont => (wf_action a /\ forall x, wf_action (cont x))
+  | ReadNondet k cont => forall x, wf_action (cont x)
+  | ReadReg r k' cont => match lookup String.eqb r regs with
+                         | None => False
+                         | Some (existT k'' _) => k' = k'' /\ forall x, wf_action (cont x)
+                         end
+  | WriteReg r k' e a => match lookup String.eqb r regs with
+                         | None => False
+                         | Some (existT k'' _) => k' = k'' /\ wf_action a
+                         end
+  | IfElse e k1 a1 a2 cont => (wf_action a1 /\ wf_action a2 /\ forall x, wf_action (cont x))
+  | Sys _ a => wf_action a
+  | Return _ => True
+  end.
+
+Fixpoint eval_ActionT{k}(meths : list (string * Signature))(updates : Updates)(a : ActionT eval_Kind k)(a_wf : wf_action a)(fs : mkProd (List.map (fun dec => eval_Kind (fst (snd dec)) -> M (eval_Kind (snd (snd dec)))) meths)){struct a} : M (Updates * eval_Kind k).
+  refine (match a return wf_action a -> _ with
+  | MCall meth s e cont => fun pf => match return_meth meth s meths fs with
                            | None => error ("Method " ++ meth ++ " not found")
                            | Some f => (
-                                io_do v <- f (eval_Expr e);
-                                eval_ActionT _ meths updates (cont v) fs
+                                do v <- f (eval_Expr e);
+                                eval_ActionT _ meths updates (cont v) _ fs
                                 )
                            end
-  | LetExpr k e cont => eval_ActionT _ meths updates (cont (eval_Expr e)) fs
-  | LetAction k a cont => (
-      io_do p <- eval_ActionT _ meths updates a fs;
-      eval_ActionT _ meths (fst p) (cont (snd p)) fs
+  | LetExpr k e cont => fun pf => eval_ActionT _ meths updates (cont (eval_Expr e)) _ fs
+  | LetAction k a cont => fun pf => (
+      do p <- eval_ActionT _ meths updates a _ fs;
+      eval_ActionT _ meths (fst p) (cont (snd p)) _ fs
       )
-  | ReadNondet k cont => (
-      io_do v <- rand_val_FK k;
-      eval_ActionT _ meths updates (cont v) fs
+  | ReadNondet k cont => fun pf => (
+      do v <- rand_val_FK k;
+      eval_ActionT _ meths updates (cont v) _ fs
       )
-  | ReadReg r k cont => match lookup String.eqb r regs with
+  | ReadReg r k cont => fun pf=> match lookup String.eqb r regs with
                         | None => reg_not_found r
                         | Some p => _
                         end
-  | WriteReg r k e a => match lookup String.eqb r regs with
+  | WriteReg r k e a => fun pf => match lookup String.eqb r regs with
                         | None => reg_not_found r
                         | Some p => _
                         end
-  | IfElse e k a1 a2 cont => let a := if (eval_Expr e) then a1 else a2 in (
-      io_do p <- eval_ActionT _ meths updates a fs;
-      eval_ActionT _ meths (fst p) (cont (snd p)) fs
+  | IfElse e k a1 a2 cont => fun pf => let a := if (eval_Expr e) then a1 else a2 in (
+      do p <- eval_ActionT _ meths updates a _ fs;
+      eval_ActionT _ meths (fst p) (cont (snd p)) _ fs
       )
-  | Sys ss a => (
-      io_do _ <- eval_list_SysT ss;
-      eval_ActionT _ meths updates a fs
+  | Sys ss a => fun pf => (
+      do _ <- eval_list_SysT ss;
+      eval_ActionT _ meths updates a _ fs
       )
-  | Return e => ret (updates, eval_Expr e)
-  end.
+  | Return e => fun pf => ret (updates, eval_Expr e)
+  end a_wf).
 Proof.
+  - apply pf.
+  - apply pf.
+  - apply pf.
+  - apply pf.
+  - apply pf.
+  (* ReadReg *)
   - destruct p.
-    destruct x.
-    * destruct k.
-      + destruct (Kind_dec2 k1 k).
-        ++ rewrite e in f.
-           exact (eval_ActionT _ meths updates (cont f) fs).
-        ++ exact (error "mismatch").
-      + exact (error "no natives").
-    * exact (error "no natives").
-  - destruct p as [x _].
-    destruct k.
-    * destruct x.
-      + destruct (Kind_dec2 k k1).
-        ++ exact (eval_ActionT _ meths ((r, existT _ (SyntaxKind k) (eval_Expr e))::updates) a fs).
-        ++ exact (error "mismatch").
-      + exact (error "no natives!!!!").
-    * exact (error "no natives").
+    simpl in pf.
+    destruct lookup in pf.
+    * destruct s; destruct pf as [keq pf'].
+      rewrite <- keq in f0.
+      exact (eval_ActionT _ meths updates (cont f0) (pf' _) fs).
+    * destruct pf.
+  (* WriteReg *)
+  - simpl in pf.
+    destruct lookup eqn:lk in pf.
+    * destruct s.
+      destruct pf as [keq pf'].
+      rewrite keq in e.
+      pose (upd := {|
+        reg_name := r;
+        kind := x;
+        old_val := f;
+        new_val := eval_Expr e;
+        lookup_match := lk
+        |}).
+      exact (eval_ActionT _ meths (upd::updates) a pf' fs).
+    * destruct pf.
+  - simpl in pf; destruct (eval_Expr e); tauto.
+  - apply pf.
+  - exact pf.
 Defined.
 
 Fixpoint curried(X : Type)(ts : list Type) : Type :=
@@ -229,83 +327,176 @@ Fixpoint curry(X : Type)(ts : list Type) : (mkProd ts -> X) -> curried X ts :=
   | T::ts' => fun f t => curry ts' (fun xs => f (t,xs))
   end.
 
-End EvalAction.
+Definition eval_RuleT(meths : list (string * Signature))(r : RuleT)(r_wf : wf_action (snd r eval_Kind))(fs : mkProd (List.map (fun dec => eval_Kind (fst (snd dec)) -> M (eval_Kind (snd (snd dec)))) meths)) : M (Updates * eval_Kind Void) :=
+  eval_ActionT meths [] ((snd r) eval_Kind) r_wf fs.
 
-Fixpoint do_single_update(upd : SimReg)(regs : SimRegs) : SimRegs :=
-  match upd with
-  | (reg,v) => match regs with
-               | [] => []
-               | (reg',v')::regs' => if String.eqb reg reg' then (reg,v)::regs' else (reg',v')::do_single_update upd regs'
-               end
+Fixpoint do_single_update(upd : Update)(regs : SimRegs) : SimRegs :=
+  match regs with
+  | [] => []
+  | (reg',v')::regs' => if String.eqb (reg_name upd) reg' then (reg', existT _ (kind upd) (new_val upd))::regs' else (reg',v')::do_single_update upd regs'
   end.
 
-Definition do_updates(upds : SimRegs)(regs : SimRegs) : SimRegs :=
+Definition do_updates(upds : Updates)(regs : SimRegs) : SimRegs :=
   fold_right do_single_update regs upds.
 
-Definition foo meths := SimRegs -> mkProd (map (fun dec : string * (Kind * Kind) => eval_Kind (fst (snd dec)) -> IO (eval_Kind (snd (snd dec)))) meths) -> IO (SimRegs * eval_Kind Void).
+End EvalAction.
 
-CoFixpoint eval_BaseModule_rr_aux(meths : list (string * Signature))(curr_regs : SimRegs)(rem_rules all_rules : list (foo meths)) : mkProd (map (fun dec : string * (Kind * Kind) => eval_Kind (fst (snd dec)) -> IO (eval_Kind (snd (snd dec)))) meths) -> IO unit :=
-  match rem_rules with
-  | [] => fun fs => bind (ret tt) (fun _ => eval_BaseModule_rr_aux curr_regs all_rules all_rules fs)
-  | a::xs => fun fs => (
-      io_do p <- a curr_regs fs;
-      eval_BaseModule_rr_aux (do_updates (fst p) curr_regs) xs all_rules fs
+Definition consistent(regs1 regs2 : SimRegs) := forall r k v,
+  lookup String.eqb r regs1 = Some (existT _ k v) -> exists v', lookup String.eqb r regs2 = Some (existT _ k v').
+
+Lemma consistent_refl : forall regs, consistent regs regs.
+Proof.
+  intros regs r k v lk.
+  exists v; auto.
+Qed.
+
+Lemma consistent_trans : forall regs1 regs2 regs3, consistent regs1 regs2 -> consistent regs2 regs3 -> consistent regs1 regs3.
+Proof.
+  intros regs1 regs2 regs3 cons12 cons23 r k v Hv.
+  destruct (cons12 r k v) as [v' Hv']; auto.
+  destruct (cons23 r k v') as [v'' Hv'']; auto.
+  exists v''; auto.
+Qed.
+
+Check lookup.
+
+Lemma lookup_cons : forall K V (eqb : K -> K -> bool) k k' v (ps : list (K*V)), lookup eqb k ((k',v)::ps) =
+  if eqb k k' then Some v else lookup eqb k ps.
+Proof.
+  intros.
+  unfold lookup.
+  unfold find.
+  simpl.
+  destruct (eqb k k'); auto.
+Qed.
+
+Lemma consistent_cons_cong : forall (regs1 regs2 : SimRegs)(r : SimReg), consistent regs1 regs2 -> consistent (r::regs1) (r::regs2).
+Proof.
+  intros regs1 regs2 r cons12 s k v Hv.
+  destruct r.
+  rewrite lookup_cons in Hv.
+  rewrite lookup_cons.
+  destruct (String.eqb s s0).
+  - exists v; auto.
+  - destruct (cons12 s k v); auto.
+    exists x; auto.
+Qed.
+
+(*
+Lemma consistent_do_update_cong : forall (regs1 regs2 : SimRegs)(upd : Update regs1),
+  consistent regs1 regs2 -> consistent (do_single_update upd regs1) (do_single_update upd regs2).
+Proof.
+Admitted.
+
+Lemma update_consistent : forall (regs : SimRegs)(upd : Update regs), consistent regs (do_single_update upd regs).
+Proof.
+  intros regs upd r k v Hv.
+  pose (lookup_match upd).
+  Print Update.
+*)
+
+Lemma wf_consistent_stable : forall {k} (a : ActionT eval_Kind k) regs1 regs2, consistent regs1 regs2 -> wf_action regs1 a -> wf_action regs2 a.
+Proof.
+  intros.
+  induction a; simpl.
+Admitted.
+
+Lemma updates_consistent : forall (regs : SimRegs)(upds : Updates regs), consistent regs (do_updates upds regs).
+Proof.
+  intros; induction upds; simpl.
+  - apply consistent_refl.
+  - apply (@consistent_trans _ (do_single_update a regs) _).
+Admitted.
+
+Lemma wf_updates_stable{k} : forall (regs : SimRegs)(upds : Updates regs)(a : ActionT eval_Kind k),
+  wf_action regs a -> wf_action (do_updates upds regs) a.
+Proof.
+  intros.
+  apply (@wf_consistent_stable _ _ regs).
+  - apply updates_consistent.
+  - auto.
+Qed.
+
+Definition maintain_wf{k} regs (upds : Updates regs) (a : ActionT eval_Kind k) : {r : RuleT & wf_action regs a} -> {r : RuleT & wf_action (do_updates upds regs) a}.
+Admitted.
+
+Fixpoint eval_Rules(timeout : nat)(meths : list (string * Signature))(init_regs : SimRegs)(rules : Stream {r : RuleT & wf_action init_regs (snd r eval_Kind)}){struct timeout} : mkProd (List.map (fun dec : string * (Kind * Kind) => eval_Kind (fst (snd dec)) -> M (eval_Kind (snd (snd dec)))) meths) -> M unit. refine
+  match timeout with
+  | 0 => fun fs => (
+      do _ <- print "TIMEOUT";
+      exit
       )
+  | S timeout' => fun fs => match rules with
+                            | Cons r rules' => (
+                                do p <- eval_RuleT init_regs meths (projT1 r) (projT2 r)  fs;
+                                eval_Rules timeout' meths (do_updates (fst p) init_regs) (Streams.map _ rules') fs
+                                )
+                            end
   end.
-
+Proof.
+  intros [rule wf].
+  exists rule.
+  apply wf_updates_stable; auto.
+Defined.
 
 Definition initialize_SimRegs(regs : list RegInitT) : SimRegs :=
-  map (fun '(r,existT k v) => match v return SimReg with
-                              | None => (r,existT _ k (eval_ConstFullT (getDefaultConstFullKind k)))
-                              | Some c => (r,existT _ k (eval_ConstFullT c))
-                              end) regs.
+  List.map (fun '(r,existT k v) => match v return SimReg with
+                                   | None => (r,existT _ k (eval_ConstFullT (getDefaultConstFullKind k)))
+                                   | Some c => (r,existT _ k (eval_ConstFullT c))
+                                   end) regs.
 
-Definition mkActionT : RuleT -> ActionT eval_Kind Void :=
-  fun '(_,a) => a eval_Kind.
+Lemma cons_neq{X}(x : X)(xs : list X) : x::xs <> [].
+Proof.
+  discriminate.
+Qed.
 
-Definition eval_BaseModule_rr_unc(meths : list (string * Signature))(m : BaseModule) :=
-  match m with
-  | BaseRegFile _ => fun _ => error "BaseRegFile not supported"
-  | BaseMod regs rules _ => let all_rules := map (fun r rgs fs => @eval_ActionT rgs Void meths [] (mkActionT r) fs) rules in eval_BaseModule_rr_aux (initialize_SimRegs regs) all_rules all_rules
+Print RuleT.
+
+Fixpoint wf_rules(regs : SimRegs)(rules : list RuleT) :=
+  match rules with
+  | [] => True
+  | r::rs => wf_action regs (snd r eval_Kind) /\ wf_rules regs rs
   end.
 
-Definition eval_BaseModule_rr meths m := curry _ (eval_BaseModule_rr_unc meths m).
+Definition wf_bm(basemod : BaseModule) : Prop :=
+  match basemod with
+  | BaseRegFile rf => False
+  | BaseMod regs rules dms => wf_rules (initialize_SimRegs regs) rules
+  end.
 
-Require Import Kami.Tutorial.SyntaxEx.
+Definition get_wf_rules : forall regs rules, wf_rules (initialize_SimRegs regs) rules -> 
+  list {r : RuleT & wf_action (initialize_SimRegs regs) (snd r eval_Kind)}.
+Proof.
+  intros.
+  induction rules.
+  - exact [].
+  - simpl in H4; destruct H4.
+    exact ((existT _ a H4)::IHrules H5).
+Defined.
 
-Section BigTest.
+Definition eval_Basemodule_rr(timeout : nat)(meths : list (string * Signature))(basemod : BaseModule)(wf : wf_bm basemod) : mkProd (List.map (fun dec : string * (Kind * Kind) => eval_Kind (fst (snd dec)) -> M (eval_Kind (snd (snd dec)))) meths) -> M unit. refine (
+  match basemod return wf_bm basemod -> _ with
+  | BaseRegFile rf => fun pf fs => _
+  | BaseMod regs rules dms =>
+      match rules with
+      | [] => fun _ _ => error "empty rules"
+      | r::rs => fun pf fs => _ (* eval_Rules timeout meths (initialize_SimRegs regs) (unwind_list (r::rs) (@cons_neq _ r rs)) *)
+      end
+  end wf).
+Proof.
+  - destruct pf.
+  - unfold wf_bm in pf.
+    refine (eval_Rules timeout meths (initialize_SimRegs regs) (unwind_list (get_wf_rules _ _ pf) _) fs).
+    simpl.
+    destruct pf; discriminate.
+Defined.
 
-Definition sigs := [("extMeth1",(Bit 20, Bool));("extMeth2",(Bit 20,Void));("extMeth3",(Void,Bit 4));("extMeth4",(Void,Void));("extMeth2_2",(Bit 20, Void))].
+Definition eval_BaseMod(timeout : nat)(meths : list (string * Signature))(basemod : BaseModule)(wf : wf_bm basemod) :=
+  curry _ (eval_Basemodule_rr timeout meths basemod wf).
 
-Definition out := eval_BaseModule_rr sigs (exampleModule "test").
+End Eval.
 
-Ltac mycbv x := let y := (eval cbv [x eval_BaseModule_rr eval_BaseModule_rr_aux eval_ActionT lookup fst find fullType Bool.eqb snd Datatypes.length curried
-  eval_list_SysT eval_SysT eval_Expr string_sigb eq_trans f_equal
-  Signature_decb String.eqb Ascii.eqb andb Kind_decb Nat.eqb
-  eq_rect_r eq_rect eq_sym orb projT1 projT2 lt_dec tup_index Fin_forallb Signature_dec2 string_dec2 Kind_dec2 Kind_decb_eq2
-  string_rec String_eqb_eq2 string_ind Kind_ind Ascii_eqb_eq2 ascii_dec Nat_eqb_eq2 Nat_eqb_refl2 nth_Fin' curry] in x) in
-  let z := eval simpl in y in
-  let w := eval cbv [eq_rect_r eq_rect eq_sym nth_Fin' nth_Fin cast Datatypes.length eq_add_S f_equal] in z in
-  let v := eval simpl in w in
-   exact w.
+Definition eval_BaseMod_Haskell := @eval_BaseMod HWord HVec IO _ _ _ _ _.
 
-Definition out2 := ltac:(mycbv out).
+Check eval_BaseMod_Haskell.
 
-End BigTest.
-
-Require Import ExtrHaskellBasic.
-Extraction Language Haskell.
-
-Extract Inductive IO => "Prelude.IO"
-
-  [
-    "Prelude.putStrLn"
-    "Prelude.return"
-    "(GHC.Base.>>=)"
-    "Prelude.error"
-    "Prelude.return (unsafeCoerce Prelude.True)" (*fix*)
-    "Prelude.return (unsafeCoerce 0)"    (*fix*)
-    "System.Exit.exitSuccess"
-  ]
-
-  "Prelude.error ""Pattern matching on IO not supported""".
