Simulator/CoqSim/CoqSimTests.v
@@ -1,0 +1,22 @@
+
+Require Import Kami.Syntax.
+Require Import Kami.Simulator.CoqSim.Eval.
+Require Import Kami.Compiler.Test.
+Require Import Kami.Simulator.NativeTest.
+Require Import Kami.Simulator.CoqSim.HaskellTypes.
+
+Definition testRegMod := snd (snd (separateModRemove testReg)).
+
+Definition timeout := 1000.
+
+Check eval_BaseMod_Haskell.
+
+Axiom cheat : forall {X},X. (* used to produce a wf proof, for now*)
+
+Definition coqSim_reg : (HWord Xlen -> IO (HWord Xlen)) -> IO unit := eval_BaseMod_Haskell timeout [("times_two", (Data,Data))] testRegMod cheat.
+
+Check separateModRemove.
+
+Definition coqSim_native : IO unit :=
+  let '(_,(_,bm)) := separateModRemove testNative in
+  eval_BaseMod_Haskell timeout [] bm cheat.
