Simulator/CoqSim/RegisterFile.v
@@ -1,0 +1,78 @@
+Require Import String.
+
+Require Import Kami.AllNotations.
+
+Require Import Kami.Simulator.CoqSim.Misc.
+Require Import Kami.Simulator.CoqSim.Eval.
+Require Import Kami.Simulator.CoqSim.SimTypes.
+
+Section RegFile.
+
+Context {V : nat -> Type -> Type}.
+Context `{IsVector V}.
+
+Context {W : nat -> Type}.
+Context `{IsWord W}.
+
+Context {M : Type -> Type -> Type}.
+Context `{IsMap M}.
+
+Definition Val k := eval_Kind W V k.
+Definition ValFK k := eval_FK W V k.
+
+Inductive FileCall :=
+  | AsyncRead : FileCall
+  | ReadReq : string -> FileCall
+  | ReadResp : string -> FileCall
+  | WriteFC : FileCall.
+
+(*
+Inductive FileUpd :=
+  | IntRegWrite : string -> Val -> FileUpd
+  | ArrWrite : string -> list (nat * Val) -> FileUpd.
+*)
+
+Record RegFile := {
+  file_name : string;
+  is_wr_mask : bool;
+  chunk_size : nat;
+  readers : RegFileReaders;
+  write : string;
+  size : nat;
+  kind : Kind;
+  arr : V size (Val kind)
+  }.
+
+Record FileState := {
+  methods : M string (FileCall * string);
+  int_regs : M string {k : FullKind & ValFK k};
+  files : M string RegFile;
+  }.
+
+Definition empty_state : FileState := {|
+  methods := empty;
+  int_regs := empty;
+  files := empty
+  |}.
+
+Check slice.
+
+Definition file_async_read(file : RegFile)(i : nat) : V (chunk_size file) (Val (kind file)) :=
+  slice i _ (arr file).
+
+(*
+Definition file_sync_readreq(file : RegFile)(v : Val Bool)(reg : string) : option (Val Bool) :=
+  match readers file with
+  | Async _ => None
+  | Sync isAddr rs => 
+  end.
+
+Definition file_sync_readreq : Val -> FileState -> RegFile -> string -> option Val. :=
+  fun val state file regName =>
+    match readers file with
+    | Async _ => cheat
+    | Sync isAddr rs => if isAddr then val else arrayVal (slice (word_to_nat (
+    end.
+*)
+
+End RegFile.
